coq_translation/default/examples/error_handling/unpacking_options_and_defaults_via_get_or_insert.v
@@ -9,7 +9,7 @@ Module Fruit.
   | Kiwi
   | Lemon.
 End Fruit.
-Definition Fruit := Fruit.t.
+Definition Fruit : Set := Fruit.t.
 
 Module
   Impl_core_fmt_Debug_for_unpacking_options_and_defaults_via_get_or_insert_Fruit.
