coq_translation/default/examples/flow_of_control/if_let_challenge.v
@@ -5,7 +5,7 @@ Module Foo.
   Inductive t : Set :=
   | Bar.
 End Foo.
-Definition Foo := Foo.t.
+Definition Foo : Set := Foo.t.
 
 (* #[allow(dead_code)] - function was ignored by the compiler *)
 Definition main `{H' : State.Trait} : M (H := H') unit :=
