coq_translation/default/examples/generics/generics_phantom_type_test_case_unit_clarification.v
@@ -5,7 +5,7 @@ Module Inch.
   Inductive t : Set :=
   .
 End Inch.
-Definition Inch := Inch.t.
+Definition Inch : Set := Inch.t.
 
 Module
   Impl_core_fmt_Debug_for_generics_phantom_type_test_case_unit_clarification_Inch.
@@ -64,7 +64,7 @@ Module Mm.
   Inductive t : Set :=
   .
 End Mm.
-Definition Mm := Mm.t.
+Definition Mm : Set := Mm.t.
 
 Module
   Impl_core_fmt_Debug_for_generics_phantom_type_test_case_unit_clarification_Mm.
